Broken commit

test.v
@@ -4,7 +4,7 @@ Inductive even : nat -> Type :=
 
 Declare ML Module "invert". 
 Lemma l1 : forall n, even (2 + n) -> even n. 
-  intros. Set Printing All.
+  intros. 
   set (diag := fun x =>                                
                  match x return Type with
                    | S (S x1) => even x1 
@@ -55,16 +55,67 @@ constructor.
 simpl. auto. 
 Qed.
 
-
-
 Section sec_absu_2ismul3.
-
 Variable C: Prop.
-
 Lemma absurd2_inv : mul3 2 -> C.
 Proof.
+set (diag := fun x => 
+               match x  with 
+                   | 0 => True
+                   | 1 => True
+                   | 2 => forall (X: Prop), X
+                   | S (S (S n)) => True
+               end). 
 intros H. 
-invert H.
+refine ((match H in mul3 k return diag k with | T0 => _ | T3 p H => _ end) _).
+simpl. auto. 
+simpl. auto. Show Proof. 
+Restart. 
+intros. 
+set (diag := fun x => 
+               match x  with 
+                   | 0 => mul3 2
+                   | 1 => mul3 2
+                   | 2 => C
+                   | S (S (S n)) => mul3 2
+               end). 
+refine ((match H in mul3 k return diag k with | T0 => _ | T3 p H => _ end)). simpl. auto. simpl. auto. 
+ Restart. 
+intros. 
+Fail invert H. 
 Abort. 
 
 End sec_absu_2ismul3.
+
+
+
+Inductive tm : Type :=
+  | const : nat -> tm
+  | plus : tm -> tm -> tm. 
+
+Inductive val : Type :=
+  | nval : nat -> val
+  | bval : bool -> val. 
+
+Inductive eval : tm -> val -> Prop :=
+| econst : forall n, eval (const n) (nval n)
+| eplus : forall t1 t2 n1 n2, eval t1 (nval n1) -> 
+                         eval t2 (nval n2) -> 
+                         eval (plus t1 t2) (nval (n1 + n2)).
+                              
+
+Goal forall v, eval (plus (const 0) (const 1)) (nval v) -> 
+          v = 1. 
+
+intros. 
+invert H. 
+set (diag := fun t (v1: val) => match t with 
+                         | const _ => v = 1
+                         | plus t1 t2 => forall (X: Prop), X
+                         end). 
+refine (match H in eval t v return diag t v with 
+          | econst _ => I
+          | eplus t1 t2 n1 n2 H1 H2 => _ end _ ) .
+simpl.  admit. 
+invert H. 
+Abort. 
